trunk/color/Term/Varyadic/VContext.v
@@ -14,134 +14,126 @@ Require Export VTerm.
 
 Section S.
 
-Variable Sig : Signature.
+  Variable Sig : Signature.
 
-Notation term := (term Sig). Notation terms := (list term).
+  Notation term := (term Sig). Notation terms := (list term).
 
 (***********************************************************************)
 (** contexts and replacement of the hole *)
 
-Inductive context : Type :=
+  Inductive context : Type :=
   | Hole : context
   | Cont : forall f : Sig, terms -> context -> terms -> context.
 
-Fixpoint fill (c : context) (t : term) : term :=
-  match c with
-    | Hole => t
-    | Cont f v1 c' v2 => Fun f (v1 ++ fill c' t :: v2)
-  end.
+  Fixpoint fill (c : context) (t : term) : term :=
+    match c with
+      | Hole => t
+      | Cont f v1 c' v2 => Fun f (v1 ++ fill c' t :: v2)
+    end.
 
-Lemma var_eq_fill : forall x c t, Var x = fill c t -> c = Hole /\ t = Var x.
+  Lemma var_eq_fill : forall x c t, Var x = fill c t -> c = Hole /\ t = Var x.
 
-Proof.
-intros. destruct c; simpl in H. auto. discr.
-Qed.
+  Proof. intros. destruct c; simpl in H. auto. discr. Qed.
 
 (***********************************************************************)
 (** context composition *)
 
-Fixpoint comp (C : context) : context -> context :=
-  match C with
-    | Hole => fun E => E
-    | Cont f ts1 D ts2 => fun E => Cont f ts1 (comp D E) ts2
-  end.
+  Fixpoint comp (C : context) : context -> context :=
+    match C with
+      | Hole => fun E => E
+      | Cont f ts1 D ts2 => fun E => Cont f ts1 (comp D E) ts2
+    end.
 
-Lemma fill_fill : forall C D u, fill C (fill D u) = fill (comp C D) u.
+  Lemma fill_fill : forall C D u, fill C (fill D u) = fill (comp C D) u.
 
-Proof.
-induction C; simpl; intros. refl. rewrite (IHC D u). refl.
-Qed.
+  Proof. induction C; simpl; intros. refl. rewrite (IHC D u). refl. Qed.
 
 (***********************************************************************)
 (** subterm ordering *)
 
-Definition subterm_eq u t := exists C, t = fill C u.
+  Definition subterm_eq u t := exists C, t = fill C u.
 
-Definition subterm u t := exists C, C <> Hole /\ t = fill C u.
+  Definition subterm u t := exists C, C <> Hole /\ t = fill C u.
 
-Lemma subterm_eq_var : forall u x, subterm_eq u (Var x) -> u = Var x.
+  Lemma subterm_eq_var : forall u x, subterm_eq u (Var x) -> u = Var x.
 
-Proof.
-intros. unfold subterm_eq in H. destruct H as [C].
-assert (C = Hole /\ u = Var x).
-apply var_eq_fill. exact H. destruct H0. exact H1.
-Qed.
+  Proof.
+    intros. unfold subterm_eq in H. destruct H as [C].
+    assert (C = Hole /\ u = Var x).
+    apply var_eq_fill. exact H. destruct H0. exact H1.
+  Qed.
 
-Lemma subterm_trans_eq2 : forall t u v,
-  subterm t u -> subterm_eq u v -> subterm t v.
+  Lemma subterm_trans_eq2 : forall t u v,
+    subterm t u -> subterm_eq u v -> subterm t v.
 
-Proof.
-unfold subterm, subterm_eq. intros. destruct H. destruct H. destruct H0.
-subst u. subst v. rewrite (fill_fill x0 x t). exists (comp x0 x).
-split. destruct x. absurd (Hole = Hole); auto.
-destruct x0; simpl; discr. refl.
-Qed.
+  Proof.
+    unfold subterm, subterm_eq. intros. destruct H. destruct H. destruct H0.
+    subst u. subst v. rewrite (fill_fill x0 x t). exists (comp x0 x).
+    split. destruct x. irrefl.
+    destruct x0; simpl; discr. refl.
+  Qed.
 
-Lemma subterm_fun_elim : forall u f ts,
-  subterm u (Fun f ts) -> exists t, In t ts /\ subterm_eq u t.
+  Lemma subterm_fun_elim : forall u f ts,
+    subterm u (Fun f ts) -> exists t, In t ts /\ subterm_eq u t.
 
-Proof.
-intros. destruct H as [C [CH fC]]. 
-destruct C. intuition.
-simpl in fC. injection fC. intros. subst ts.
-exists (fill C u). split. auto with datatypes.
-unfold subterm_eq. exists C. refl.
-Qed.
+  Proof.
+    intros. destruct H as [C [CH fC]]. 
+    destruct C. intuition.
+    simpl in fC. injection fC. intros. subst ts.
+    exists (fill C u). split. auto with datatypes.
+    unfold subterm_eq. exists C. refl.
+  Qed.
 
-Lemma subterm_immediate : forall f v a, In a v -> subterm a (Fun f v).
+  Lemma subterm_immediate : forall f v a, In a v -> subterm a (Fun f v).
 
-Proof.
-  intros. destruct (In_split a v) as [l1 [l2 dec]]. hyp.
-  exists (Cont f l1 Hole l2). split. discr. simpl. congruence.
-Qed.
+  Proof.
+    intros. destruct (In_split a v) as [l1 [l2 dec]]. hyp.
+    exists (Cont f l1 Hole l2). split. discr. simpl. congruence.
+  Qed.
 
 (***********************************************************************)
 (** subterm-based induction principle *)
 
-Lemma subterm_eq_rect : forall (P : term -> Type) t,
-  (forall u, subterm_eq u t -> P u) -> P t.
+  Lemma subterm_eq_rect : forall (P : term -> Type) t,
+    (forall u, subterm_eq u t -> P u) -> P t.
 
-Proof.
-  intros. apply X. unfold subterm_eq. exists Hole. auto.
-Qed.
+  Proof. intros. apply X. unfold subterm_eq. exists Hole. auto. Qed.
 
-Require Import ListForall.
+  Require Import ListForall.
 
-Lemma subterm_sub_ind : forall (P : term -> Prop)
-  (IH : forall t, (forall u, subterm u t -> P u) -> P t),
-  forall t u, subterm_eq u t -> P u.
+  Lemma subterm_sub_ind : forall (P : term -> Prop)
+    (IH : forall t, (forall u, subterm u t -> P u) -> P t),
+    forall t u, subterm_eq u t -> P u.
 
-Proof.
-intros P IH. set (P' := fun t => forall u, subterm_eq u t -> P u).
-change (forall t, P' t). apply term_ind_forall.
-(* var *)
-unfold P'. intros. assert (u = Var x). apply subterm_eq_var. hyp.
-subst u. apply IH. unfold subterm. intros. destruct H0. destruct H0.
-destruct x0. absurd (Hole = Hole); auto. discr.
-(* fun *)
-intros. unfold P'. intros. apply IH. intros.
-assert (subterm u0 (Fun f v)). eapply subterm_trans_eq2. apply H1. hyp.
-assert (exists t, In t v /\ subterm_eq u0 t). apply subterm_fun_elim with f.
-hyp.
-destruct H3. destruct H3.
-assert (P' x). apply lforall_in with term v. hyp. hyp.
-apply H5. hyp.
-Qed.
+  Proof.
+    intros P IH. set (P' := fun t => forall u, subterm_eq u t -> P u).
+    change (forall t, P' t). apply term_ind_forall.
+    (* var *)
+    unfold P'. intros. assert (u = Var x). apply subterm_eq_var. hyp.
+    subst u. apply IH. unfold subterm. intros. destruct H0. destruct H0.
+    destruct x0. irrefl. discr.
+    (* fun *)
+    intros. unfold P'. intros. apply IH. intros.
+    assert (subterm u0 (Fun f v)). eapply subterm_trans_eq2. apply H1. hyp.
+    assert (exists t, In t v /\ subterm_eq u0 t). apply subterm_fun_elim with f.
+    hyp.
+    destruct H3. destruct H3.
+    assert (P' x). apply lforall_in with term v. hyp. hyp.
+    apply H5. hyp.
+  Qed.
 
-Lemma subterm_ind : forall (P : term -> Prop)
-  (IH : forall t, (forall u, subterm u t -> P u) -> P t),
-  forall t, P t.
+  Lemma subterm_ind : forall (P : term -> Prop)
+    (IH : forall t, (forall u, subterm u t -> P u) -> P t),
+    forall t, P t.
 
-Proof.
-  intros. apply subterm_eq_rect. apply subterm_sub_ind. hyp.
-Qed.
+  Proof. intros. apply subterm_eq_rect. apply subterm_sub_ind. hyp. Qed.
 
-Lemma subterm_wf : well_founded subterm.
+  Lemma subterm_wf : well_founded subterm.
 
-Proof.
-  intro t. induction t using subterm_ind. constructor. intros.
-  apply H. hyp.
-Qed.
+  Proof.
+    intro t. induction t using subterm_ind. constructor. intros.
+    apply H. hyp.
+  Qed.
 
 End S.
 
